updates

high2/Zeta.High.Interleave.fsti
@@ -33,22 +33,26 @@ let vlog_ext_of_il_log (#app: app_params) (#n:nat)
   : seq (vlog_entry_ext app)
   = IF.map mk_vlog_entry_ext il
 
-let is_eac #app #n (il: verifiable_log app n)
-  = eac (vlog_ext_of_il_log il)
+val is_eac (#app #n:_) (il: verifiable_log app n)
+  : b:bool{b <==> eac (vlog_ext_of_il_log il)}
 
 let eac_log (app: app_params) (n:nat) = il: verifiable_log app n {is_eac il}
 
 let neac_log (app: app_params) (n:nat) = il: verifiable_log app n {~ (is_eac il)}
 
-val eac_boundary (#app #n:_) (il: verifiable_log app n)
+val eac_boundary (#app #n:_) (il: neac_log app n)
   : (i: seq_index il{is_eac (prefix il i) /\
                      ~ (is_eac (prefix il (i+1)))})
 
 val lemma_eac_implies_prefix_eac (#app #n:_) (il: eac_log app n) (i: nat{i <= S.length il})
   : Lemma (ensures (is_eac (prefix il i)))
 
-(*val lemma_eac_implies_appfn_valid (#app #n:_) (il: eac_log app n)
-  : Lemma (ensures (let rs = GI.appfn_calls #(high_verifier_spec app) #n il in
-                    True))
-*)
-  //Zeta.AppSimulate.valid_call_result (appfn_calls il)))
+#push-options "--z3rlimit_factor 3"
+// TODO: why (high_verifier_spec app).app == app is so hard to infer?
+let appfn_calls (#app #n:_) (il: eac_log app n)
+  : seq (Zeta.AppSimulate.appfn_call_res app)
+  = GI.appfn_calls il
+#pop-options
+
+val lemma_eac_implies_appfn_valid (#app #n:_) (il: eac_log app n)
+  : Lemma (ensures (Zeta.AppSimulate.valid_call_result (appfn_calls il)))
