high2/Zeta.High.Interleave.fst
@@ -1,0 +1,25 @@
+module Zeta.High.Interleave
+
+let mk_vlog_entry_ext (#app: app_params) (#n:nat)
+  : IF.idxfn_t (gen_seq app n) (vlog_entry_ext app)
+  = admit()
+
+let is_eac_post (#app: app_params) (#n:nat)
+  (il: verifiable_log app n) (i: seq_index il)
+  : bool
+  = let il' = prefix il (i+1) in
+    let l' = vlog_ext_of_il_log il' in
+    is_eac_log l'
+
+let is_eac #app #n (il: verifiable_log app n)
+  = is_eac_log (vlog_ext_of_il_log il)
+
+let lemma_eac_empty #app #n (il: verifiable_log app n{S.length il = 0})
+  : Lemma (ensures (is_eac il))
+  = let le = vlog_ext_of_il_log il in
+    eac_empty_log le
+
+let eac_boundary (#app #n:_) (il: neac_log app n)
+  : (i: seq_index il{is_eac (prefix il i) /\
+                     ~ (is_eac (prefix il (i+1)))})
+  = admit()
