utils/Zeta.IdxFn.fsti
@@ -249,6 +249,14 @@ val lemma_filter_map_monotonic
   (s: gs.seq_t)
   : Lemma (ensures (filter_map (FM (conj fm.f f) fm.m) s == filter_map fm (gs.prefix s (flen f s))))
 
+val lemma_map_prefix
+  (#gs:_)
+  (#b:_)
+  (f: idxfn_t gs b)
+  (s: gs.seq_t)
+  (i:nat{i <= gs.length s})
+  : Lemma (ensures (SA.prefix (map f s) i == map f (gs.prefix s i)))
+
 let seq_basic (a:eqtype) : gen_seq_spec = {
   seq_t = seq a;
   length;
